tests/elab/implicitReducibilityForDSimprocs.lean
@@ -1,3 +1,11 @@
+import Lean.Meta.Basic
+import Lean.Elab.Tactic.Basic
+
+syntax (name := Lean.Parser.Tactic.withImplicit) "with_implicit " tacticSeq : tactic
+
+@[tactic Lean.Parser.Tactic.withImplicit] def evalWithImplicit : Lean.Elab.Tactic.Tactic := fun stx =>
+  Lean.Meta.withImplicit <| Lean.Elab.Tactic.evalTactic stx[1]
+
 set_option allowUnsafeReducibility true in
 attribute [implicit_reducible]
   Char.ofNat Char.ofNatAux
@@ -59,187 +67,187 @@ attribute [implicit_reducible]
 
 section Array
 
-example : #[1, 2, 3][1] = 2 := by with_reducible_and_instances rfl
-example : #[1, 2, 3][1]? = some 2 := by with_reducible_and_instances rfl
-example : #[1, 2, 3][1]! = 2 := by with_reducible_and_instances rfl
+example : #[1, 2, 3][1] = 2 := by with_implicit rfl
+example : #[1, 2, 3][1]? = some 2 := by with_implicit rfl
+example : #[1, 2, 3][1]! = 2 := by with_implicit rfl
 
 end Array
 
 section BitVec
 
-example : - 0#3 = 0#3 := by with_reducible_and_instances rfl
-example : ~~~ 0#3 = -1#3 := by with_reducible_and_instances rfl
-example : BitVec.abs (-1#3) = 1#3 := by with_reducible_and_instances rfl
-example : 3#3 &&& 5#3 = 1#3 := by with_reducible_and_instances rfl
-example : 3#3 ||| 5#3 = 7#3 := by with_reducible_and_instances rfl
-example : 3#3 ^^^ 5#3 = 6#3 := by with_reducible_and_instances rfl
-example : 3#8 + 5#8 = 8#8 := by with_reducible_and_instances rfl
-example : 5#8 - 3#8 = 2#8 := by with_reducible_and_instances rfl
-example : 3#8 * 5#8 = 15#8 := by with_reducible_and_instances rfl
-example : 13#8 / 5#8 = 2#8 := by with_reducible_and_instances rfl
-example : 13#8 % 5#8 = 3#8 := by with_reducible_and_instances rfl
-example : BitVec.udiv 13#8 5#8 = 2#8 := by with_reducible_and_instances rfl
-example : BitVec.umod 13#8 5#8 = 3#8 := by with_reducible_and_instances rfl
-example : BitVec.smtUDiv 13#8 5#8 = 2#8 := by with_reducible_and_instances rfl
-example : BitVec.smod 13#8 5#8 = 3#8 := by with_reducible_and_instances rfl
-example : BitVec.srem 13#8 5#8 = 3#8 := by with_reducible_and_instances rfl
-example : BitVec.sdiv 13#8 5#8 = 2#8 := by with_reducible_and_instances rfl
-example : BitVec.smtSDiv 13#8 5#8 = 2#8 := by with_reducible_and_instances rfl
-example : BitVec.getLsbD 13#8 0 = true := by with_reducible_and_instances rfl
-example : BitVec.getMsbD 13#8 0 = false := by with_reducible_and_instances rfl
-example : BitVec.clz 13#8 = 4#8 := by with_reducible_and_instances rfl
-example : BitVec.cpop 13#8 = 3#8 := by with_reducible_and_instances rfl
-example : (13#8)[0] = true := by with_reducible_and_instances rfl
-example : BitVec.shiftLeft 13#8 1 = 26#8 := by with_reducible_and_instances rfl
-example : BitVec.ushiftRight 13#8 1 = 6#8 := by with_reducible_and_instances rfl
-example : BitVec.sshiftRight 13#8 1 = 6#8 := by with_reducible_and_instances rfl
-example : 13#8 <<< 1 = 26#8 := by with_reducible_and_instances rfl
-example : 13#8 <<< 1#3 = 26#8 := by with_reducible_and_instances rfl
-example : 13#8 >>> 1 = 6#8 := by with_reducible_and_instances rfl
-example : 13#8 >>> 1#3 = 6#8 := by with_reducible_and_instances rfl
-example : BitVec.rotateLeft 13#8 1 = 26#8 := by with_reducible_and_instances rfl
-example : BitVec.rotateRight 13#8 1 = 134#8 := by with_reducible_and_instances rfl
-example : 1#4 ++ 1#4 = 17#8 := by with_reducible_and_instances rfl
+example : - 0#3 = 0#3 := by with_implicit rfl
+example : ~~~ 0#3 = -1#3 := by with_implicit rfl
+example : BitVec.abs (-1#3) = 1#3 := by with_implicit rfl
+example : 3#3 &&& 5#3 = 1#3 := by with_implicit rfl
+example : 3#3 ||| 5#3 = 7#3 := by with_implicit rfl
+example : 3#3 ^^^ 5#3 = 6#3 := by with_implicit rfl
+example : 3#8 + 5#8 = 8#8 := by with_implicit rfl
+example : 5#8 - 3#8 = 2#8 := by with_implicit rfl
+example : 3#8 * 5#8 = 15#8 := by with_implicit rfl
+example : 13#8 / 5#8 = 2#8 := by with_implicit rfl
+example : 13#8 % 5#8 = 3#8 := by with_implicit rfl
+example : BitVec.udiv 13#8 5#8 = 2#8 := by with_implicit rfl
+example : BitVec.umod 13#8 5#8 = 3#8 := by with_implicit rfl
+example : BitVec.smtUDiv 13#8 5#8 = 2#8 := by with_implicit rfl
+example : BitVec.smod 13#8 5#8 = 3#8 := by with_implicit rfl
+example : BitVec.srem 13#8 5#8 = 3#8 := by with_implicit rfl
+example : BitVec.sdiv 13#8 5#8 = 2#8 := by with_implicit rfl
+example : BitVec.smtSDiv 13#8 5#8 = 2#8 := by with_implicit rfl
+example : BitVec.getLsbD 13#8 0 = true := by with_implicit rfl
+example : BitVec.getMsbD 13#8 0 = false := by with_implicit rfl
+example : BitVec.clz 13#8 = 4#8 := by with_implicit rfl
+example : BitVec.cpop 13#8 = 3#8 := by with_implicit rfl
+example : (13#8)[0] = true := by with_implicit rfl
+example : BitVec.shiftLeft 13#8 1 = 26#8 := by with_implicit rfl
+example : BitVec.ushiftRight 13#8 1 = 6#8 := by with_implicit rfl
+example : BitVec.sshiftRight 13#8 1 = 6#8 := by with_implicit rfl
+example : 13#8 <<< 1 = 26#8 := by with_implicit rfl
+example : 13#8 <<< 1#3 = 26#8 := by with_implicit rfl
+example : 13#8 >>> 1 = 6#8 := by with_implicit rfl
+example : 13#8 >>> 1#3 = 6#8 := by with_implicit rfl
+example : BitVec.rotateLeft 13#8 1 = 26#8 := by with_implicit rfl
+example : BitVec.rotateRight 13#8 1 = 134#8 := by with_implicit rfl
+example : 1#4 ++ 1#4 = 17#8 := by with_implicit rfl
 -- TODO: test case for `reduceCast`?
-example : (13#8).toNat = 13 := by with_reducible_and_instances rfl
-example : (13#8).toInt = 13 := by with_reducible_and_instances rfl
-example : BitVec.ofInt 8 13 = 13#8 := by with_reducible_and_instances rfl
-example : BitVec.ofNat 8 13 = 13#8 := by with_reducible_and_instances rfl
-example : (13#8 == 12#8) = false := by with_reducible_and_instances rfl
-example : (13#8 != 12#8) = true := by with_reducible_and_instances rfl
-example : BitVec.ult 12#8 13#8 = true := by with_reducible_and_instances rfl
-example : BitVec.ule 12#8 13#8 = true := by with_reducible_and_instances rfl
-example : BitVec.slt (-1#8) (0#8) = true := by with_reducible_and_instances rfl
-example : BitVec.sle (-1#8) (0#8) = true := by with_reducible_and_instances rfl
-example : BitVec.setWidth' (show 2 ≤ 4 by grind) 1#2 = 1#4 := by with_reducible_and_instances rfl
-example : BitVec.shiftLeftZeroExtend 13#8 1 = 26#9 := by with_reducible_and_instances rfl
-example : BitVec.extractLsb' 1 1 13#8 = 0#1 := by with_reducible_and_instances rfl
-example : BitVec.replicate 8 1#1 = 255#8 := by with_reducible_and_instances rfl
-example : BitVec.setWidth 4 13#8 = 13#4 := by with_reducible_and_instances rfl
-example : BitVec.zeroExtend 8 15#4 = 15#8 := by with_reducible_and_instances rfl
-example : BitVec.signExtend 8 15#4 = 255#8 := by with_reducible_and_instances rfl
-example : BitVec.allOnes 8 = 255#8 := by with_reducible_and_instances rfl
-example : BitVec.ofFin (Fin.mk 3 (show 3 < 2 ^ 8 by grind)) = 3#8 := by with_reducible_and_instances rfl
-example : BitVec.toFin 3#8 = Fin.mk 3 (show 3 < 2 ^ 8 by grind) := by with_reducible_and_instances rfl
+example : (13#8).toNat = 13 := by with_implicit rfl
+example : (13#8).toInt = 13 := by with_implicit rfl
+example : BitVec.ofInt 8 13 = 13#8 := by with_implicit rfl
+example : BitVec.ofNat 8 13 = 13#8 := by with_implicit rfl
+example : (13#8 == 12#8) = false := by with_implicit rfl
+example : (13#8 != 12#8) = true := by with_implicit rfl
+example : BitVec.ult 12#8 13#8 = true := by with_implicit rfl
+example : BitVec.ule 12#8 13#8 = true := by with_implicit rfl
+example : BitVec.slt (-1#8) (0#8) = true := by with_implicit rfl
+example : BitVec.sle (-1#8) (0#8) = true := by with_implicit rfl
+example : BitVec.setWidth' (show 2 ≤ 4 by grind) 1#2 = 1#4 := by with_implicit rfl
+example : BitVec.shiftLeftZeroExtend 13#8 1 = 26#9 := by with_implicit rfl
+example : BitVec.extractLsb' 1 1 13#8 = 0#1 := by with_implicit rfl
+example : BitVec.replicate 8 1#1 = 255#8 := by with_implicit rfl
+example : BitVec.setWidth 4 13#8 = 13#4 := by with_implicit rfl
+example : BitVec.zeroExtend 8 15#4 = 15#8 := by with_implicit rfl
+example : BitVec.signExtend 8 15#4 = 255#8 := by with_implicit rfl
+example : BitVec.allOnes 8 = 255#8 := by with_implicit rfl
+example : BitVec.ofFin (Fin.mk 3 (show 3 < 2 ^ 8 by grind)) = 3#8 := by with_implicit rfl
+example : BitVec.toFin 3#8 = Fin.mk 3 (show 3 < 2 ^ 8 by grind) := by with_implicit rfl
 
 end BitVec
 
 section Char
 
-example : 'A'.toLower = 'a' := by with_reducible_and_instances rfl
-example : 'a'.toUpper = 'A' := by with_reducible_and_instances rfl
-example : 'A'.toNat = 65 := by with_reducible_and_instances rfl
-example : ' '.isWhitespace = true := by with_reducible_and_instances rfl
-example : 'A'.isUpper = true := by with_reducible_and_instances rfl
-example : 'a'.isLower = true := by with_reducible_and_instances rfl
-example : 'a'.isAlpha = true := by with_reducible_and_instances rfl
-example : '5'.isDigit = true := by with_reducible_and_instances rfl
-example : '5'.isAlphanum = true := by with_reducible_and_instances rfl
-example : toString 'A' = "A" := by with_reducible_and_instances rfl
-example : 'A'.val = 65 := by with_reducible_and_instances rfl
-example : ('A' == 'B') = false := by with_reducible_and_instances rfl
-example : ('A' != 'B') = true := by with_reducible_and_instances rfl
-example : Char.ofNat 65 = 'A' := by with_reducible_and_instances rfl
-example : Char.ofNatAux 65 (by decide) = 'A' := by with_reducible_and_instances rfl
-example : (default : Char) = 'A' := by with_reducible_and_instances rfl
+example : 'A'.toLower = 'a' := by with_implicit rfl
+example : 'a'.toUpper = 'A' := by with_implicit rfl
+example : 'A'.toNat = 65 := by with_implicit rfl
+example : ' '.isWhitespace = true := by with_implicit rfl
+example : 'A'.isUpper = true := by with_implicit rfl
+example : 'a'.isLower = true := by with_implicit rfl
+example : 'a'.isAlpha = true := by with_implicit rfl
+example : '5'.isDigit = true := by with_implicit rfl
+example : '5'.isAlphanum = true := by with_implicit rfl
+example : toString 'A' = "A" := by with_implicit rfl
+example : 'A'.val = 65 := by with_implicit rfl
+example : ('A' == 'B') = false := by with_implicit rfl
+example : ('A' != 'B') = true := by with_implicit rfl
+example : Char.ofNat 65 = 'A' := by with_implicit rfl
+example : Char.ofNatAux 65 (by decide) = 'A' := by with_implicit rfl
+example : (default : Char) = 'A' := by with_implicit rfl
 
 -- This is the `rfl` lemma `Char.toNat_val`.
-example (c : Char) : c.val.toNat = c.toNat := by with_reducible_and_instances rfl
+example (c : Char) : c.val.toNat = c.toNat := by with_implicit rfl
 
 end Char
 
 section Fin
 
-example : (2 : Fin 5).succ = 3 := by with_reducible_and_instances rfl
-example : (2 : Fin 5).rev = 2 := by with_reducible_and_instances rfl
-example : Fin.last 5 = 5 := by with_reducible_and_instances rfl
-example : (2 : Fin 5) + 3 = 0 := by with_reducible_and_instances rfl
-example : (2 : Fin 5) * 3 = 1 := by with_reducible_and_instances rfl
-example : (3 : Fin 5) - 1 = 2 := by with_reducible_and_instances rfl
-example : (4 : Fin 5) / 2 = 2 := by with_reducible_and_instances rfl
-example : (4 : Fin 5) % 3 = 1 := by with_reducible_and_instances rfl
-example : (3 : Fin 8) &&& 5 = 1 := by with_reducible_and_instances rfl
-example : (3 : Fin 8) ||| 5 = 7 := by with_reducible_and_instances rfl
-example : (3 : Fin 8) ^^^ 5 = 6 := by with_reducible_and_instances rfl
-example : (3 : Fin 8) <<< (1 : Fin 8) = 6 := by with_reducible_and_instances rfl
-example : (4 : Fin 8) >>> (1 : Fin 8) = 2 := by with_reducible_and_instances rfl
-example : ((3 : Fin 5) == 3) = true := by with_reducible_and_instances rfl
-example : ((3 : Fin 5) != 4) = true := by with_reducible_and_instances rfl
-example : (3 : Fin 5) = ⟨3, by decide⟩ := by with_reducible_and_instances rfl
-example : (Fin.mk 3 (by decide) : Fin 5) = 3 := by with_reducible_and_instances rfl
-example : Fin.ofNat 5 3 = (3 : Fin 5) := by with_reducible_and_instances rfl
-example : Fin.castSucc (3 : Fin 5) = 3 := by with_reducible_and_instances rfl
-example : Fin.castAdd 3 (2 : Fin 5) = 2 := by with_reducible_and_instances rfl
-example : Fin.addNat (2 : Fin 5) 3 = 5 := by with_reducible_and_instances rfl
-example : Fin.natAdd 3 (2 : Fin 5) = 5 := by with_reducible_and_instances rfl
-example : Fin.castLT (2 : Fin 5) (by decide) = (2 : Fin 3) := by with_reducible_and_instances rfl
-example : Fin.castLE (show 5 ≤ 8 by decide) (2 : Fin 5) = 2 := by with_reducible_and_instances rfl
-example : Fin.subNat 2 (5 : Fin 8) (by decide) = 3 := by with_reducible_and_instances rfl
-example : Fin.pred (3 : Fin 6) (by decide) = 2 := by with_reducible_and_instances rfl
+example : (2 : Fin 5).succ = 3 := by with_implicit rfl
+example : (2 : Fin 5).rev = 2 := by with_implicit rfl
+example : Fin.last 5 = 5 := by with_implicit rfl
+example : (2 : Fin 5) + 3 = 0 := by with_implicit rfl
+example : (2 : Fin 5) * 3 = 1 := by with_implicit rfl
+example : (3 : Fin 5) - 1 = 2 := by with_implicit rfl
+example : (4 : Fin 5) / 2 = 2 := by with_implicit rfl
+example : (4 : Fin 5) % 3 = 1 := by with_implicit rfl
+example : (3 : Fin 8) &&& 5 = 1 := by with_implicit rfl
+example : (3 : Fin 8) ||| 5 = 7 := by with_implicit rfl
+example : (3 : Fin 8) ^^^ 5 = 6 := by with_implicit rfl
+example : (3 : Fin 8) <<< (1 : Fin 8) = 6 := by with_implicit rfl
+example : (4 : Fin 8) >>> (1 : Fin 8) = 2 := by with_implicit rfl
+example : ((3 : Fin 5) == 3) = true := by with_implicit rfl
+example : ((3 : Fin 5) != 4) = true := by with_implicit rfl
+example : (3 : Fin 5) = ⟨3, by decide⟩ := by with_implicit rfl
+example : (Fin.mk 3 (by decide) : Fin 5) = 3 := by with_implicit rfl
+example : Fin.ofNat 5 3 = (3 : Fin 5) := by with_implicit rfl
+example : Fin.castSucc (3 : Fin 5) = 3 := by with_implicit rfl
+example : Fin.castAdd 3 (2 : Fin 5) = 2 := by with_implicit rfl
+example : Fin.addNat (2 : Fin 5) 3 = 5 := by with_implicit rfl
+example : Fin.natAdd 3 (2 : Fin 5) = 5 := by with_implicit rfl
+example : Fin.castLT (2 : Fin 5) (by decide) = (2 : Fin 3) := by with_implicit rfl
+example : Fin.castLE (show 5 ≤ 8 by decide) (2 : Fin 5) = 2 := by with_implicit rfl
+example : Fin.subNat 2 (5 : Fin 8) (by decide) = 3 := by with_implicit rfl
+example : Fin.pred (3 : Fin 6) (by decide) = 2 := by with_implicit rfl
 
 end Fin
 
 section List
 
-example : List.replicate 3 5 = [5, 5, 5] := by with_reducible_and_instances rfl
+example : List.replicate 3 5 = [5, 5, 5] := by with_implicit rfl
 
 end List
 
 section String
 
-example : "abc" ++ "def" = "abcdef" := by with_reducible_and_instances rfl
-example : String.ofList ['a', 'b', 'c'] = "abc" := by with_reducible_and_instances rfl
-example : "abc".toList = ['a', 'b', 'c'] := by with_reducible_and_instances rfl
-example : "ab".push 'c' = "abc" := by with_reducible_and_instances rfl
-example : String.singleton 'A' = "A" := by with_reducible_and_instances rfl
-example : "A" = String.singleton 'A' := by with_reducible_and_instances rfl
-example : ("A" == "B") = false := by with_reducible_and_instances rfl
-example : ("A" != "B") = true := by with_reducible_and_instances rfl
+example : "abc" ++ "def" = "abcdef" := by with_implicit rfl
+example : String.ofList ['a', 'b', 'c'] = "abc" := by with_implicit rfl
+example : "abc".toList = ['a', 'b', 'c'] := by with_implicit rfl
+example : "ab".push 'c' = "abc" := by with_implicit rfl
+example : String.singleton 'A' = "A" := by with_implicit rfl
+example : "A" = String.singleton 'A' := by with_implicit rfl
+example : ("A" == "B") = false := by with_implicit rfl
+example : ("A" != "B") = true := by with_implicit rfl
 
 end String
 
 section Nat
 
-example : 3 + 5 = 8 := by with_reducible_and_instances rfl
-example : 5 - 3 = 2 := by with_reducible_and_instances rfl
-example : 3 * 5 = 15 := by with_reducible_and_instances rfl
-example : 13 / 5 = 2 := by with_reducible_and_instances rfl
-example : 13 % 5 = 3 := by with_reducible_and_instances rfl
-example : 3 ^ 2 = 9 := by with_reducible_and_instances rfl
-example : 3 &&& 5 = 1 := by with_reducible_and_instances rfl
-example : 3 ||| 5 = 7 := by with_reducible_and_instances rfl
-example : 3 ^^^ 5 = 6 := by with_reducible_and_instances rfl
-example : 3 <<< 1 = 6 := by with_reducible_and_instances rfl
-example : 3 >>> 1 = 1 := by with_reducible_and_instances rfl
-example : Nat.gcd 10 15 = 5 := by with_reducible_and_instances rfl
-example : (13 == 12) = false := by with_reducible_and_instances rfl
-example : (13 != 12) = true := by with_reducible_and_instances rfl
+example : 3 + 5 = 8 := by with_implicit rfl
+example : 5 - 3 = 2 := by with_implicit rfl
+example : 3 * 5 = 15 := by with_implicit rfl
+example : 13 / 5 = 2 := by with_implicit rfl
+example : 13 % 5 = 3 := by with_implicit rfl
+example : 3 ^ 2 = 9 := by with_implicit rfl
+example : 3 &&& 5 = 1 := by with_implicit rfl
+example : 3 ||| 5 = 7 := by with_implicit rfl
+example : 3 ^^^ 5 = 6 := by with_implicit rfl
+example : 3 <<< 1 = 6 := by with_implicit rfl
+example : 3 >>> 1 = 1 := by with_implicit rfl
+example : Nat.gcd 10 15 = 5 := by with_implicit rfl
+example : (13 == 12) = false := by with_implicit rfl
+example : (13 != 12) = true := by with_implicit rfl
 
 end Nat
 
 section Int
 
-example : -(-3) = (3 : Int) := by with_reducible_and_instances rfl
-example : 3 + 5 = (8 : Int) := by with_reducible_and_instances rfl
-example : 5 - 3 = (2 : Int) := by with_reducible_and_instances rfl
-example : 3 * 5 = (15 : Int) := by with_reducible_and_instances rfl
-example : 13 / 5 = (2 : Int) := by with_reducible_and_instances rfl
-example : Int.tdiv 13 5 = (2 : Int) := by with_reducible_and_instances rfl
-example : Int.fdiv 13 5 = (2 : Int) := by with_reducible_and_instances rfl
-example : Int.bdiv 13 5 = (3 : Int) := by with_reducible_and_instances rfl
-example : 13 % 5 = (3 : Int) := by with_reducible_and_instances rfl
-example : Int.tmod 13 5 = (3 : Int) := by with_reducible_and_instances rfl
-example : Int.fmod 13 5 = (3 : Int) := by with_reducible_and_instances rfl
-example : Int.bmod 13 5 = (-2 : Int) := by with_reducible_and_instances rfl
-example : 3 ^ 2 = (9 : Int) := by with_reducible_and_instances rfl
-example : ((13 : Int) == 12) = false := by with_reducible_and_instances rfl
-example : ((13 : Int) != 12) = true := by with_reducible_and_instances rfl
-example : Int.natAbs (-5) = 5 := by with_reducible_and_instances rfl
-example : Int.toNat (-5) = 0 := by with_reducible_and_instances rfl
-example : Int.negSucc 2 = -3 := by with_reducible_and_instances rfl
-example : Int.ofNat 3 = 3 := by with_reducible_and_instances rfl
-example : NatCast.natCast 3 = (3 : Int) := by with_reducible_and_instances rfl
-example : Nat.cast 3 = (3 : Int) := by with_reducible_and_instances rfl
+example : -(-3) = (3 : Int) := by with_implicit rfl
+example : 3 + 5 = (8 : Int) := by with_implicit rfl
+example : 5 - 3 = (2 : Int) := by with_implicit rfl
+example : 3 * 5 = (15 : Int) := by with_implicit rfl
+example : 13 / 5 = (2 : Int) := by with_implicit rfl
+example : Int.tdiv 13 5 = (2 : Int) := by with_implicit rfl
+example : Int.fdiv 13 5 = (2 : Int) := by with_implicit rfl
+example : Int.bdiv 13 5 = (3 : Int) := by with_implicit rfl
+example : 13 % 5 = (3 : Int) := by with_implicit rfl
+example : Int.tmod 13 5 = (3 : Int) := by with_implicit rfl
+example : Int.fmod 13 5 = (3 : Int) := by with_implicit rfl
+example : Int.bmod 13 5 = (-2 : Int) := by with_implicit rfl
+example : 3 ^ 2 = (9 : Int) := by with_implicit rfl
+example : ((13 : Int) == 12) = false := by with_implicit rfl
+example : ((13 : Int) != 12) = true := by with_implicit rfl
+example : Int.natAbs (-5) = 5 := by with_implicit rfl
+example : Int.toNat (-5) = 0 := by with_implicit rfl
+example : Int.negSucc 2 = -3 := by with_implicit rfl
+example : Int.ofNat 3 = 3 := by with_implicit rfl
+example : NatCast.natCast 3 = (3 : Int) := by with_implicit rfl
+example : Nat.cast 3 = (3 : Int) := by with_implicit rfl
 
 end Int
 
@@ -249,133 +257,133 @@ section SInt
 arithmetic.
 We need to make sure that these are `rfl` at implicit transparency.
 -/
-example : Int8.minValue.toInt = - 2 ^ 7 := by with_reducible_and_instances rfl
-example : Int16.minValue.toInt = - 2 ^ 15 := by with_reducible_and_instances rfl
-example : Int32.minValue.toInt = - 2 ^ 31 := by with_reducible_and_instances rfl
-example : Int64.minValue.toInt = - 2 ^ 63 := by with_reducible_and_instances rfl
+example : Int8.minValue.toInt = - 2 ^ 7 := by with_implicit rfl
+example : Int16.minValue.toInt = - 2 ^ 15 := by with_implicit rfl
+example : Int32.minValue.toInt = - 2 ^ 31 := by with_implicit rfl
+example : Int64.minValue.toInt = - 2 ^ 63 := by with_implicit rfl
 
-example : 3 * 5 = (15 : Int8) := by with_reducible_and_instances rfl
-example : 3 * 5 = (15 : Int16) := by with_reducible_and_instances rfl
-example : 3 * 5 = (15 : Int32) := by with_reducible_and_instances rfl
-example : 3 * 5 = (15 : Int64) := by with_reducible_and_instances rfl
+example : 3 * 5 = (15 : Int8) := by with_implicit rfl
+example : 3 * 5 = (15 : Int16) := by with_implicit rfl
+example : 3 * 5 = (15 : Int32) := by with_implicit rfl
+example : 3 * 5 = (15 : Int64) := by with_implicit rfl
 
-example : 3 + 5 = (8 : Int8) := by with_reducible_and_instances rfl
-example : 3 + 5 = (8 : Int16) := by with_reducible_and_instances rfl
-example : 3 + 5 = (8 : Int32) := by with_reducible_and_instances rfl
-example : 3 + 5 = (8 : Int64) := by with_reducible_and_instances rfl
+example : 3 + 5 = (8 : Int8) := by with_implicit rfl
+example : 3 + 5 = (8 : Int16) := by with_implicit rfl
+example : 3 + 5 = (8 : Int32) := by with_implicit rfl
+example : 3 + 5 = (8 : Int64) := by with_implicit rfl
 
-example : 3 - 5 = (-2 : Int8) := by with_reducible_and_instances rfl
-example : 3 - 5 = (-2 : Int16) := by with_reducible_and_instances rfl
-example : 3 - 5 = (-2 : Int32) := by with_reducible_and_instances rfl
-example : 3 - 5 = (-2 : Int64) := by with_reducible_and_instances rfl
+example : 3 - 5 = (-2 : Int8) := by with_implicit rfl
+example : 3 - 5 = (-2 : Int16) := by with_implicit rfl
+example : 3 - 5 = (-2 : Int32) := by with_implicit rfl
+example : 3 - 5 = (-2 : Int64) := by with_implicit rfl
 
-example : 13 / 5 = (2 : Int8) := by with_reducible_and_instances rfl
-example : 13 / 5 = (2 : Int16) := by with_reducible_and_instances rfl
-example : 13 / 5 = (2 : Int32) := by with_reducible_and_instances rfl
-example : 13 / 5 = (2 : Int64) := by with_reducible_and_instances rfl
+example : 13 / 5 = (2 : Int8) := by with_implicit rfl
+example : 13 / 5 = (2 : Int16) := by with_implicit rfl
+example : 13 / 5 = (2 : Int32) := by with_implicit rfl
+example : 13 / 5 = (2 : Int64) := by with_implicit rfl
 
-example : 13 % 5 = (3 : Int8) := by with_reducible_and_instances rfl
-example : 13 % 5 = (3 : Int16) := by with_reducible_and_instances rfl
-example : 13 % 5 = (3 : Int32) := by with_reducible_and_instances rfl
-example : 13 % 5 = (3 : Int64) := by with_reducible_and_instances rfl
+example : 13 % 5 = (3 : Int8) := by with_implicit rfl
+example : 13 % 5 = (3 : Int16) := by with_implicit rfl
+example : 13 % 5 = (3 : Int32) := by with_implicit rfl
+example : 13 % 5 = (3 : Int64) := by with_implicit rfl
 
 section
 set_option warn.sorry false
-example : (13 : Int8) = Int8.ofIntLE 13 sorry sorry := by with_reducible_and_instances rfl
-example : (13 : Int16) = Int16.ofIntLE 13 sorry sorry := by with_reducible_and_instances rfl
-example : (13 : Int32) = Int32.ofIntLE 13 sorry sorry := by with_reducible_and_instances rfl
-example : (13 : Int64) = Int64.ofIntLE 13 sorry sorry := by with_reducible_and_instances rfl
+example : (13 : Int8) = Int8.ofIntLE 13 sorry sorry := by with_implicit rfl
+example : (13 : Int16) = Int16.ofIntLE 13 sorry sorry := by with_implicit rfl
+example : (13 : Int32) = Int32.ofIntLE 13 sorry sorry := by with_implicit rfl
+example : (13 : Int64) = Int64.ofIntLE 13 sorry sorry := by with_implicit rfl
 end
 
-example : (13 : Int8) = Int8.ofNat 13 := by with_reducible_and_instances rfl
-example : (13 : Int16) = Int16.ofNat 13 := by with_reducible_and_instances rfl
-example : (13 : Int32) = Int32.ofNat 13 := by with_reducible_and_instances rfl
-example : (13 : Int64) = Int64.ofNat 13 := by with_reducible_and_instances rfl
+example : (13 : Int8) = Int8.ofNat 13 := by with_implicit rfl
+example : (13 : Int16) = Int16.ofNat 13 := by with_implicit rfl
+example : (13 : Int32) = Int32.ofNat 13 := by with_implicit rfl
+example : (13 : Int64) = Int64.ofNat 13 := by with_implicit rfl
 
-example : (13 : Nat) = (13 : Int8).toNatClampNeg := by with_reducible_and_instances rfl
-example : (0 : Nat) = (-13 : Int8).toNatClampNeg := by with_reducible_and_instances rfl
-example : (13 : Nat) = (13 : Int16).toNatClampNeg := by with_reducible_and_instances rfl
-example : (0 : Nat) = (-13 : Int16).toNatClampNeg := by with_reducible_and_instances rfl
-example : (13 : Nat) = (13 : Int32).toNatClampNeg := by with_reducible_and_instances rfl
-example : (0 : Nat) = (-13 : Int32).toNatClampNeg := by with_reducible_and_instances rfl
-example : (13 : Nat) = (13 : Int64).toNatClampNeg := by with_reducible_and_instances rfl
-example : (0 : Nat) = (-13 : Int64).toNatClampNeg := by with_reducible_and_instances rfl
+example : (13 : Nat) = (13 : Int8).toNatClampNeg := by with_implicit rfl
+example : (0 : Nat) = (-13 : Int8).toNatClampNeg := by with_implicit rfl
+example : (13 : Nat) = (13 : Int16).toNatClampNeg := by with_implicit rfl
+example : (0 : Nat) = (-13 : Int16).toNatClampNeg := by with_implicit rfl
+example : (13 : Nat) = (13 : Int32).toNatClampNeg := by with_implicit rfl
+example : (0 : Nat) = (-13 : Int32).toNatClampNeg := by with_implicit rfl
+example : (13 : Nat) = (13 : Int64).toNatClampNeg := by with_implicit rfl
+example : (0 : Nat) = (-13 : Int64).toNatClampNeg := by with_implicit rfl
 
-example : (-13 : Int8) = Int8.ofInt (-13) := by with_reducible_and_instances rfl
-example : (-13 : Int16) = Int16.ofInt (-13) := by with_reducible_and_instances rfl
-example : (-13 : Int32) = Int32.ofInt (-13) := by with_reducible_and_instances rfl
-example : (-13 : Int64) = Int64.ofInt (-13) := by with_reducible_and_instances rfl
+example : (-13 : Int8) = Int8.ofInt (-13) := by with_implicit rfl
+example : (-13 : Int16) = Int16.ofInt (-13) := by with_implicit rfl
+example : (-13 : Int32) = Int32.ofInt (-13) := by with_implicit rfl
+example : (-13 : Int64) = Int64.ofInt (-13) := by with_implicit rfl
 
-example : (-13 : Int) = (-13 : Int8).toInt := by with_reducible_and_instances rfl
-example : (-13 : Int) = (-13 : Int16).toInt := by with_reducible_and_instances rfl
-example : (-13 : Int) = (-13 : Int32).toInt := by with_reducible_and_instances rfl
-example : (-13 : Int) = (-13 : Int64).toInt := by with_reducible_and_instances rfl
+example : (-13 : Int) = (-13 : Int8).toInt := by with_implicit rfl
+example : (-13 : Int) = (-13 : Int16).toInt := by with_implicit rfl
+example : (-13 : Int) = (-13 : Int32).toInt := by with_implicit rfl
+example : (-13 : Int) = (-13 : Int64).toInt := by with_implicit rfl
 
 end SInt
 
 section UInt
 
-example : 3 * 5 = (15 : UInt8) := by with_reducible_and_instances rfl
-example : 3 * 5 = (15 : UInt16) := by with_reducible_and_instances rfl
-example : 3 * 5 = (15 : UInt32) := by with_reducible_and_instances rfl
-example : 3 * 5 = (15 : UInt64) := by with_reducible_and_instances rfl
+example : 3 * 5 = (15 : UInt8) := by with_implicit rfl
+example : 3 * 5 = (15 : UInt16) := by with_implicit rfl
+example : 3 * 5 = (15 : UInt32) := by with_implicit rfl
+example : 3 * 5 = (15 : UInt64) := by with_implicit rfl
 
-example : 3 + 5 = (8 : UInt8) := by with_reducible_and_instances rfl
-example : 3 + 5 = (8 : UInt16) := by with_reducible_and_instances rfl
-example : 3 + 5 = (8 : UInt32) := by with_reducible_and_instances rfl
-example : 3 + 5 = (8 : UInt64) := by with_reducible_and_instances rfl
+example : 3 + 5 = (8 : UInt8) := by with_implicit rfl
+example : 3 + 5 = (8 : UInt16) := by with_implicit rfl
+example : 3 + 5 = (8 : UInt32) := by with_implicit rfl
+example : 3 + 5 = (8 : UInt64) := by with_implicit rfl
 
-example : 5 - 3 = (2 : UInt8) := by with_reducible_and_instances rfl
-example : 5 - 3 = (2 : UInt16) := by with_reducible_and_instances rfl
-example : 5 - 3 = (2 : UInt32) := by with_reducible_and_instances rfl
-example : 5 - 3 = (2 : UInt64) := by with_reducible_and_instances rfl
+example : 5 - 3 = (2 : UInt8) := by with_implicit rfl
+example : 5 - 3 = (2 : UInt16) := by with_implicit rfl
+example : 5 - 3 = (2 : UInt32) := by with_implicit rfl
+example : 5 - 3 = (2 : UInt64) := by with_implicit rfl
 
-example : 13 / 5 = (2 : UInt8) := by with_reducible_and_instances rfl
-example : 13 / 5 = (2 : UInt16) := by with_reducible_and_instances rfl
-example : 13 / 5 = (2 : UInt32) := by with_reducible_and_instances rfl
-example : 13 / 5 = (2 : UInt64) := by with_reducible_and_instances rfl
+example : 13 / 5 = (2 : UInt8) := by with_implicit rfl
+example : 13 / 5 = (2 : UInt16) := by with_implicit rfl
+example : 13 / 5 = (2 : UInt32) := by with_implicit rfl
+example : 13 / 5 = (2 : UInt64) := by with_implicit rfl
 
-example : 13 % 5 = (3 : UInt8) := by with_reducible_and_instances rfl
-example : 13 % 5 = (3 : UInt16) := by with_reducible_and_instances rfl
-example : 13 % 5 = (3 : UInt32) := by with_reducible_and_instances rfl
-example : 13 % 5 = (3 : UInt64) := by with_reducible_and_instances rfl
+example : 13 % 5 = (3 : UInt8) := by with_implicit rfl
+example : 13 % 5 = (3 : UInt16) := by with_implicit rfl
+example : 13 % 5 = (3 : UInt32) := by with_implicit rfl
+example : 13 % 5 = (3 : UInt64) := by with_implicit rfl
 
-example : (13 : UInt8) = UInt8.ofNat 13 := by with_reducible_and_instances rfl
-example : (13 : UInt16) = UInt16.ofNat 13 := by with_reducible_and_instances rfl
-example : (13 : UInt32) = UInt32.ofNat 13 := by with_reducible_and_instances rfl
-example : (13 : UInt64) = UInt64.ofNat 13 := by with_reducible_and_instances rfl
+example : (13 : UInt8) = UInt8.ofNat 13 := by with_implicit rfl
+example : (13 : UInt16) = UInt16.ofNat 13 := by with_implicit rfl
+example : (13 : UInt32) = UInt32.ofNat 13 := by with_implicit rfl
+example : (13 : UInt64) = UInt64.ofNat 13 := by with_implicit rfl
 
-example : (13 : Nat) = (13 : UInt8).toNat := by with_reducible_and_instances rfl
-example : (13 : Nat) = (13 : UInt16).toNat := by with_reducible_and_instances rfl
-example : (13 : Nat) = (13 : UInt32).toNat := by with_reducible_and_instances rfl
-example : (13 : Nat) = (13 : UInt64).toNat := by with_reducible_and_instances rfl
+example : (13 : Nat) = (13 : UInt8).toNat := by with_implicit rfl
+example : (13 : Nat) = (13 : UInt16).toNat := by with_implicit rfl
+example : (13 : Nat) = (13 : UInt32).toNat := by with_implicit rfl
+example : (13 : Nat) = (13 : UInt64).toNat := by with_implicit rfl
 
-example : ((13 : UInt8) == 12) = false := by with_reducible_and_instances rfl
-example : ((13 : UInt8) != 12) = true := by with_reducible_and_instances rfl
-example : ((13 : UInt16) == 12) = false := by with_reducible_and_instances rfl
-example : ((13 : UInt16) != 12) = true := by with_reducible_and_instances rfl
-example : ((13 : UInt32) == 12) = false := by with_reducible_and_instances rfl
-example : ((13 : UInt32) != 12) = true := by with_reducible_and_instances rfl
-example : ((13 : UInt64) == 12) = false := by with_reducible_and_instances rfl
-example : ((13 : UInt64) != 12) = true := by with_reducible_and_instances rfl
+example : ((13 : UInt8) == 12) = false := by with_implicit rfl
+example : ((13 : UInt8) != 12) = true := by with_implicit rfl
+example : ((13 : UInt16) == 12) = false := by with_implicit rfl
+example : ((13 : UInt16) != 12) = true := by with_implicit rfl
+example : ((13 : UInt32) == 12) = false := by with_implicit rfl
+example : ((13 : UInt32) != 12) = true := by with_implicit rfl
+example : ((13 : UInt64) == 12) = false := by with_implicit rfl
+example : ((13 : UInt64) != 12) = true := by with_implicit rfl
 
 section
 set_option warn.sorry false
-example : UInt8.ofNatLT 13 sorry = 13 := by with_reducible_and_instances rfl
-example : UInt16.ofNatLT 13 sorry = 13 := by with_reducible_and_instances rfl
-example : UInt32.ofNatLT 13 sorry = 13 := by with_reducible_and_instances rfl
-example : UInt64.ofNatLT 13 sorry = 13 := by with_reducible_and_instances rfl
+example : UInt8.ofNatLT 13 sorry = 13 := by with_implicit rfl
+example : UInt16.ofNatLT 13 sorry = 13 := by with_implicit rfl
+example : UInt32.ofNatLT 13 sorry = 13 := by with_implicit rfl
+example : UInt64.ofNatLT 13 sorry = 13 := by with_implicit rfl
 end
 
-example : UInt8.ofNat 13 = 13 := by with_reducible_and_instances rfl
-example : UInt16.ofNat 13 = 13 := by with_reducible_and_instances rfl
-example : UInt32.ofNat 13 = 13 := by with_reducible_and_instances rfl
-example : UInt64.ofNat 13 = 13 := by with_reducible_and_instances rfl
+example : UInt8.ofNat 13 = 13 := by with_implicit rfl
+example : UInt16.ofNat 13 = 13 := by with_implicit rfl
+example : UInt32.ofNat 13 = 13 := by with_implicit rfl
+example : UInt64.ofNat 13 = 13 := by with_implicit rfl
 
-example : UInt8.toNat 13 = 13 := by with_reducible_and_instances rfl
-example : UInt16.toNat 13 = 13 := by with_reducible_and_instances rfl
-example : UInt32.toNat 13 = 13 := by with_reducible_and_instances rfl
-example : UInt64.toNat 13 = 13 := by with_reducible_and_instances rfl
+example : UInt8.toNat 13 = 13 := by with_implicit rfl
+example : UInt16.toNat 13 = 13 := by with_implicit rfl
+example : UInt32.toNat 13 = 13 := by with_implicit rfl
+example : UInt64.toNat 13 = 13 := by with_implicit rfl
 
 end UInt
 
